theory/x64Assembler.thy
@@ -199,6 +199,12 @@ fun x64_encode :: "instruction \<Rightarrow> x64_bin option" where
     let (op::u8) = 0x87 in
     let (rop::u8) = construct_modsib_to_u8 0b11 (u8_of_ireg r1) (u8_of_ireg rd) in
       Some [rex, op, rop] |
+  \<comment> \<open> P2878 `CDQ : sign_extend_eax_edx `   -> ` 1001 1001 ` \<close>  
+  Pcdq \<Rightarrow>
+    Some [0x99] |
+  \<comment> \<open> P2878 `CQO : sign_extend_rax_rdx `   -> ` 0100 1001 1001 1001 ` \<close>
+  Pcqo \<Rightarrow>
+    Some [0x48, 0x99] |
   \<comment> \<open> P2876 `ADD register1 to register2` -> `0100 0R0B : 0000 000w : 11 reg1 reg2` \<close>
   Paddl_rr rd r1 \<Rightarrow>
     let (rex:: u8) = (construct_rex_to_u8  \<comment> \<open> `0R0B` \<close>
@@ -221,7 +227,7 @@ fun x64_encode :: "instruction \<Rightarrow> x64_bin option" where
       False \<comment> \<open> X \<close>
       (and (u8_of_ireg rd) 0b1000 \<noteq> 0) \<comment> \<open> B \<close>
       ) in
-    let (op:: u8) = 0x01 in
+    let (op:: u8) = 0x81 in
     let (rop::u8) = construct_modsib_to_u8 0b11 0b000 (u8_of_ireg rd) in
     if rex = 0x40 then
       Some ([op, rop] @ u8_list_of_u32 n) 
@@ -277,6 +283,20 @@ fun x64_encode :: "instruction \<Rightarrow> x64_bin option" where
         Some [ op, rop ] 
       else 
         Some [ rex, op, rop ] |
+ \<comment> \<open> P2891 `SUB: immediate from register` -> `0100 000B 1000 00sw : 11 101 reg : imm` \<close>
+  Psubl_ri rd n \<Rightarrow>
+    let (rex:: u8) = (construct_rex_to_u8  \<comment> \<open> `000B` \<close>
+      False \<comment> \<open> W \<close>
+      False \<comment> \<open> R \<close>
+      False \<comment> \<open> X \<close>
+      (and (u8_of_ireg rd) 0b1000 \<noteq> 0) \<comment> \<open> B \<close>
+      ) in
+    let (op:: u8) = 0x81 in
+    let (rop::u8) = construct_modsib_to_u8 0b11 0b101 (u8_of_ireg rd) in
+      if rex = 0x40 then
+        Some ([op, rop] @ u8_list_of_u32 n) 
+      else 
+        Some  ([rex, op, rop] @ u8_list_of_u32 n) |
   \<comment> \<open> P2884 `NEG register2` -> `0100 100B : 1111 0111 : 11011reg` \<close>
   Pnegq rd \<Rightarrow>
     let (rex:: u8) = (construct_rex_to_u8  \<comment> \<open> `100B` \<close>
@@ -290,7 +310,7 @@ fun x64_encode :: "instruction \<Rightarrow> x64_bin option" where
       Some [rex, op, rop ] |
   \<comment> \<open> P2884 `OR register1 to register2` -> ` 0000 100w : 11 reg1 reg2` \<close>
   Porl_rr rd r1  \<Rightarrow> 
-     let (rex:: u8) = (construct_rex_to_u8  \<comment> \<open> `1R0B` \<close>
+     let (rex:: u8) = (construct_rex_to_u8  \<comment> \<open> `0R0B` \<close>
       False \<comment> \<open> W \<close>
       (and (u8_of_ireg r1) 0b1000 \<noteq> 0) \<comment> \<open> R \<close>
       False \<comment> \<open> X \<close>
@@ -313,6 +333,20 @@ fun x64_encode :: "instruction \<Rightarrow> x64_bin option" where
     let (op:: u8) = 0x09 in
     let (rop::u8) = construct_modsib_to_u8 0b11 (u8_of_ireg r1) (u8_of_ireg rd) in
       Some [ rex, op, rop] |
+ \<comment> \<open> P2891 `OR: immediate to register` -> `0100 000B  1000 00sw : 11 001 reg : imm` \<close>
+  Porl_ri rd n \<Rightarrow>
+    let (rex:: u8) = (construct_rex_to_u8  \<comment> \<open> `000B` \<close>
+      False \<comment> \<open> W \<close>
+      False \<comment> \<open> R \<close>
+      False \<comment> \<open> X \<close>
+      (and (u8_of_ireg rd) 0b1000 \<noteq> 0) \<comment> \<open> B \<close>
+      ) in
+    let (op:: u8) = 0x81 in
+    let (rop::u8) = construct_modsib_to_u8 0b11 0b001 (u8_of_ireg rd) in
+      if rex = 0x40 then
+        Some ([op, rop] @ u8_list_of_u32 n) 
+      else 
+        Some  ([rex, op, rop] @ u8_list_of_u32 n) |
   \<comment> \<open> P2876 `AND register1 to register2` -> ` 0100 0R0B : 0010 000w : 11 reg1 reg2` \<close>
   Pandl_rr rd r1  \<Rightarrow> 
      let (rex:: u8) = (construct_rex_to_u8  \<comment> \<open> `0R0B` \<close>
@@ -338,6 +372,20 @@ fun x64_encode :: "instruction \<Rightarrow> x64_bin option" where
     let (op:: u8) = 0x21 in
     let (rop::u8) = construct_modsib_to_u8 0b11 (u8_of_ireg r1) (u8_of_ireg rd) in
       Some [ rex, op, rop] |
+ \<comment> \<open> P2891 `AND: immediate to register` -> `0100 000B : 1000 00sw : 11 100 reg : immediate` \<close>
+  Pandl_ri rd n \<Rightarrow>
+    let (rex:: u8) = (construct_rex_to_u8  \<comment> \<open> `000B` \<close>
+      False \<comment> \<open> W \<close>
+      False \<comment> \<open> R \<close>
+      False \<comment> \<open> X \<close>
+      (and (u8_of_ireg rd) 0b1000 \<noteq> 0) \<comment> \<open> B \<close>
+      ) in
+    let (op:: u8) = 0x81 in
+    let (rop::u8) = construct_modsib_to_u8 0b11 0b100 (u8_of_ireg rd) in
+      if rex = 0x40 then
+        Some ([op, rop] @ u8_list_of_u32 n) 
+      else 
+        Some  ([rex, op, rop] @ u8_list_of_u32 n) |
   \<comment> \<open> P2893 `XOR register1 to register2` -> ` 0100 0RXB : 0011 000w : 11 reg1 reg2` \<close>
   Pxorl_rr rd r1  \<Rightarrow> 
      let (rex:: u8) = (construct_rex_to_u8  \<comment> \<open> `0R0B` \<close>
@@ -363,6 +411,20 @@ fun x64_encode :: "instruction \<Rightarrow> x64_bin option" where
     let (op:: u8) = 0x31 in
     let (rop::u8) = construct_modsib_to_u8 0b11 (u8_of_ireg r1) (u8_of_ireg rd) in
       Some [ rex, op, rop] |
+  \<comment> \<open> P2893 `XOR: immediate to register` -> ` 0100 000B 1000 00sw : 11 110 reg : imm` \<close>
+  Pxorl_ri rd n \<Rightarrow>
+    let (rex:: u8) = (construct_rex_to_u8  \<comment> \<open> `000B` \<close>
+      False \<comment> \<open> W \<close>
+      False \<comment> \<open> R \<close>
+      False \<comment> \<open> X \<close>
+      (and (u8_of_ireg rd) 0b1000 \<noteq> 0) \<comment> \<open> B \<close>
+      ) in
+    let (op:: u8) = 0x81 in
+    let (rop::u8) = construct_modsib_to_u8 0b11 0b110 (u8_of_ireg rd) in
+      if rex = 0x40 then
+        Some ([op, rop] @ u8_list_of_u32 n) 
+      else 
+        Some  ([rex, op, rop] @ u8_list_of_u32 n) |
   \<comment> \<open> P2884 `MUL AL, AX, or EAX with register2` -> ` 0100 000B : 1111 011w : 11 100 reg` \<close>
   Pmull_r r1 \<Rightarrow>
     let (rex:: u8) = (construct_rex_to_u8  \<comment> \<open> `000B` \<close>
@@ -831,6 +893,9 @@ fun x64_encode :: "instruction \<Rightarrow> x64_bin option" where
   Pcall_i d  \<Rightarrow>
     let (op::u8) = 0xe8 in
       Some [op,(ucast (and d 0xff)),(ucast (d >> 8)),(ucast (d >> 16)),(ucast (d >> 24))]|
+  \<comment> \<open> P2887 ` RET near`   -> ` 1100 0011` \<close>
+  Pret \<Rightarrow>
+    Some [0xc3]|
   \<comment> \<open> P2884 `NOP – No Operation` -> `1001 0000` \<close>
   Pnop \<Rightarrow> Some [0x90] |
   _ \<Rightarrow> None
